added substituition to Logic.lean and made Assign_example.lean

Hoare/Logic.lean
@@ -5,11 +5,43 @@ namespace Hoare
 open While
 
 -- TODO: define substitution properly
-axiom _root_.Statement.subst :  String → Expr → Statement → Statement
+--axiom _root_.Statement.subst :  String → Expr → Statement → Statement
+
+-- Not really sure if this is capture-avoiding subsitution, it was the most
+-- naive thing to try. 
+
+def Expr.subst (x : String) (e : Expr) (e' : Expr) : Expr :=
+  match e' with
+  | Expr.var y => if x == y then e else e'
+  | Expr.num n => Expr.num n
+  | Expr.bool b => Expr.bool b
+  | Expr.add e1 e2 => Expr.add (Expr.subst x e e1) (Expr.subst x e e2)
+  | Expr.sub e1 e2 => Expr.sub (Expr.subst x e e1) (Expr.subst x e e2)
+  | Expr.mul e1 e2 => Expr.mul (Expr.subst x e e1) (Expr.subst x e e2)
+  | Expr.eq e1 e2 => Expr.eq (Expr.subst x e e1) (Expr.subst x e e2)
+  | Expr.lt e1 e2 => Expr.lt (Expr.subst x e e1) (Expr.subst x e e2)
+  | Expr.gt e1 e2 => Expr.gt (Expr.subst x e e1) (Expr.subst x e e2)
+  | Expr.le e1 e2 => Expr.le (Expr.subst x e e1) (Expr.subst x e e2)
+  | Expr.ge e1 e2 => Expr.ge (Expr.subst x e e1) (Expr.subst x e e2)
+  | Expr.and e1 e2 => Expr.and (Expr.subst x e e1) (Expr.subst x e e2)
+  | Expr.or e1 e2 => Expr.or (Expr.subst x e e1) (Expr.subst x e e2)
+
+def Statement.subst (x : String) (e : Expr) (P : Statement) : Statement :=
+  match P with
+  | Statement.atom expr => Statement.atom (Expr.subst x e expr)
+  | Statement.conj P₁ P₂ => Statement.conj (Statement.subst x e P₁) (Statement.subst x e P₂)
+  | Statement.disj P₁ P₂ => Statement.disj (Statement.subst x e P₁) (Statement.subst x e P₂)
+  | Statement.neg P' => Statement.neg (Statement.subst x e P')
+  | Statement.impl P₁ P₂ => Statement.impl (Statement.subst x e P₁) (Statement.subst x e P₂)
+  | Statement.equiv P₁ P₂ => Statement.equiv (Statement.subst x e P₁) (Statement.subst x e P₂)
 
 inductive TripleHolds : Triple → Prop
   | skip {P : Statement} {c : Com} : TripleHolds {$(P)} $(c) {$(P)} --{P:= P, c := Com.skip, Q := P}
-  | assign {P : Statement} {e : Expr} {x : String} {c : Com} : TripleHolds {$(P)} $(c) {$(P.subst x e)}
+  | assign {P : Statement} {e : Expr} {x : String} {c : Com} : TripleHolds {$(Statement.subst x e P)} $(c) {$(P)}
+  -- for some reason I had a lot of inference problems with assign using curly braces,
+  -- so I have added assign' which makes all parameters explicit and with assign prime I am
+  -- able to prove hoare triple statment in Assign_example.lean
+  | assign' (P : Statement) (e : Expr) (x : String) (c : Com) : TripleHolds {$(Statement.subst x e P)} $(c) {$(P)}
   | seq {P Q R : Statement} {c₁ c₂ : Com} :
       TripleHolds {$(P)} $(c₁) {$(Q)} → TripleHolds {$(Q)} $(c₂) {$(R)} →
       TripleHolds {$(P)} $(c₁);$(c₂) {$(Q)}
