Hoare/Examples/Assign_example.lean
@@ -1,0 +1,28 @@
+import Hoare.While
+import Hoare.Logic
+import Hoare.Statements
+
+open Hoare While
+
+
+
+def foo : Triple :=
+{(X + 1) == 2}
+X := X + 1
+{X == 2}
+
+def foo_com : Com := [com| X := X + 1]
+
+def foo_expr : Expr := [expr| X + 1]
+
+def foo_stmt : Statement := Statement.atom [expr| X == 2]
+
+theorem foo_match  : Statement.subst "X" foo_expr foo_stmt = [stmt| (X + 1) == 2] := by
+  simp [foo_expr, foo_stmt, Statement.subst]
+  simp [Expr.subst]
+
+-- Here we use TripleHolds.assign' I had some inference problems getting TripleHolds.assign
+-- to work.
+theorem foo_holds' : TripleHolds foo := by
+  have := TripleHolds.assign' foo_stmt foo_expr "X" foo_com
+  exact this
